4[\{x,a\}, \{a,b\}, \{b,c\}]
5[\{x,a\}, \{a,b\}, \{x,c\}]
6[\{x,a\}, \{a,b\}, \{a,c\}]
7[\{x,a\}, \{x,b\}, \{x,c\}]
8[\{x,a\}, \{a,b\}, \{b,c\}, \{x,c\}]
9[\{x,a\}, \{a,b\}, \{b,c\}, \{a,c\}]
10[\{x,a\}, \{a,b\}, \{a,c\}, \{x,c\}]
11[\{x,a\}, \{x,b\}, \{a,c\}, \{x,c\}]
12[\{x,a\}, \{a,b\}, \{b,c\}, \{a,c\}, \{x,c\}]
13[\{x,a\}, \{b,c\}, \{x,b\}, \{a,c\}, \{x,c\}]
14[\{x,a\}, \{a,b\}, \{b,c\}, \{x,b\}, \{a,c\}, \{x,c\}]

\[o_{15} + 2o_{27} + 2o_{34} + 2o_{35} + 2o_{45} + o_{51} + 2o_{52} + o_{59} = \sum\limits_{x,t,u,v:P_{4} (x,t,u,v)} ( c( v ) - 1 ) \]
\[o_{16} + o_{29} + 2o_{34} + 2o_{36} + 2o_{46} + o_{51} + 2o_{52} + o_{59} = \sum\limits_{x,t,u,v:P_{4} (x,t,u,v)} ( c( x ) - 1 ) \]
\[2o_{17} + 2o_{30} + 2o_{34} + o_{37} + o_{48} + o_{51} + o_{53} + o_{60} = \sum\limits_{x,t,u,v:P_{5} (x,t,u,v)} ( c( v ) - 1 ) \]
\[2o_{18} + o_{24} + 2o_{27} + 2o_{36} + 2o_{45} + 2o_{46} + o_{51} + o_{59} = \sum\limits_{x,t,u,v:P_{4} (x,t,u,v)} ( c( u ) - 2 ) \]
\[o_{19} + 2o_{31} + 2o_{35} + o_{37} + 2o_{39} + o_{40} + 4o_{49} + 4o_{54} = \sum\limits_{x,t,u,v:P_{6} (x,t,u,v)} ( c( u ) - 1 ) + ( c( v ) - 1 ) \]
\[o_{20} + o_{32} + o_{37} + o_{40} + 2o_{49} + 2o_{54} = \sum\limits_{x,t,u,v:P_{6} (x,t,u,v)} ( c( x ) - 1 ) \]
\[2o_{21} + o_{26} + 2o_{30} + 2o_{38} + 2o_{47} + o_{48} + o_{53} + o_{60} = \sum\limits_{x,t,u,v:P_{5} (x,t,u,v)} ( c( x ) - 2 ) \]
\[3o_{22} + 2o_{31} + o_{32} + o_{39} + o_{40} + 2o_{54} = \sum\limits_{x,t,u,v:P_{6} (x,t,u,v)} ( c( t ) - 3 ) \]
\[4o_{23} + 2o_{33} + o_{42} + o_{55} = \sum\limits_{x,t,u,v:P_{7} (x,t,u,v)} ( c( x ) - 3 ) \]
\[o_{24} + 2o_{45} + 2o_{46} + o_{59} = \sum\limits_{x,t,u,v:P_{4} (x,t,u,v)} c( t, u ) \]
\[2o_{25} + o_{40} + o_{48} + 2o_{52} + 2o_{57} + o_{59} + 2o_{64} + 2o_{66} = \sum\limits_{x,t,u,v:P_{10} (x,t,u,v)} ( c( v ) - 2 ) \]
\[o_{26} + 2o_{47} + o_{48} + o_{60} = \sum\limits_{x,t,u,v:P_{5} (x,t,u,v)} c( x, t ) \]
\[2o_{27} + 2o_{45} + o_{51} + o_{59} = \sum\limits_{x,t,u,v:P_{4} (x,t,u,v)} c( u, v ) \]
\[o_{28} + o_{43} + o_{51} + o_{59} + 2o_{62} + 2o_{65} = \sum\limits_{x,t,u,v:P_{9} (x,t,u,v)} ( c( x ) - 1 ) \]
\[o_{29} + 2o_{43} + 2o_{52} + o_{53} + o_{59} + o_{60} + 2o_{64} + 2o_{66} = \sum\limits_{x,t,u,v:P_{10} (x,t,u,v)} ( c( u ) - 1 ) \]
\[o_{30} + 4o_{44} + o_{53} + 2o_{61} + o_{63} + o_{67} = \sum\limits_{x,t,u,v:P_{11} (x,t,u,v)} ( c( u ) - 1 ) \]
\[o_{31} + 2o_{39} + o_{43} + 3o_{56} + o_{59} + 2o_{65} = \sum\limits_{x,t,u,v:P_{9} (x,t,u,v)} ( c( t ) - 3 ) \]
\[o_{32} + o_{40} + 2o_{54} = \sum\limits_{x,t,u,v:P_{6} (x,t,u,v)} c( x, t ) \]
\[2o_{33} + 2o_{42} + 4o_{44} + 3o_{58} + 2o_{61} + o_{67} = \sum\limits_{x,t,u,v:P_{11} (x,t,u,v)} ( c( x ) - 3 ) \]
\[2o_{34} + o_{51} + 2o_{52} + o_{59} = \sum\limits_{x,t,u,v:P_{4} (x,t,u,v)} c( x, v ) \]
\[2o_{35} + 2o_{45} + 2o_{52} + o_{59} = \sum\limits_{x,t,u,v:P_{4} (x,t,u,v)} ( c( t, v ) - 1 ) \]
\[o_{36} + 3o_{50} + o_{51} + 2o_{62} + 2o_{63} + o_{68} = \sum\limits_{x,t,u,v:P_{8} (x,t,u,v)} ( c( u ) - 2 ) \]
\[o_{37} + o_{40} + 4o_{49} + 4o_{54} = \sum\limits_{x,t,u,v:P_{6} (x,t,u,v)} ( c( x, u ) - 1 ) + ( c( x, v ) - 1 ) \]
\[o_{38} + 3o_{50} + o_{53} + 2o_{63} + o_{64} + o_{68} = \sum\limits_{x,t,u,v:P_{8} (x,t,u,v)} ( c( x ) - 2 ) \]
\[2o_{39} + 6o_{56} + o_{59} + 4o_{65} = \sum\limits_{x,t,u,v:P_{9} (x,t,u,v)} ( c( t, u ) - 1 ) + ( c( t, v ) - 1 ) \]
\[o_{40} + 4o_{54} + o_{59} + o_{60} + 4o_{65} + 2o_{66} + 2o_{68} + 6o_{70} = \sum\limits_{x,t,u,v:P_{12} (x,t,u,v)} ( c( t ) - 3 ) + ( c( v ) - 3 ) \]
\[o_{41} + 3o_{55} + o_{60} + 2o_{67} + o_{68} + 2o_{71} = \sum\limits_{x,t,u,v:P_{13} (x,t,u,v)} ( c( v ) - 3 ) \]
\[o_{42} + 3o_{55} = \sum\limits_{x,t,u,v:P_{7} (x,t,u,v)} c( x, t, u ) + c( x, t, v ) + c( x, u, v ) \]
\[o_{43} + o_{59} + 2o_{65} = \sum\limits_{x,t,u,v:P_{9} (x,t,u,v)} c( x, t ) \]
\[4o_{44} + 2o_{61} + o_{67} = \sum\limits_{x,t,u,v:P_{11} (x,t,u,v)} c( x, u ) \]
\[2o_{45} + o_{59} = \sum\limits_{x,t,u,v:P_{4} (x,t,u,v)} c( t, u, v ) \]
\[o_{46} + o_{59} + o_{63} + 2o_{65} + 2o_{68} + 3o_{70} = \sum\limits_{x,t,u,v:P_{12} (x,t,u,v)} ( c( u ) - 2 ) \]
\[o_{47} + 3o_{58} + o_{63} + o_{67} = \sum\limits_{x,t,u,v:P_{11} (x,t,u,v)} ( c( t, v ) - 1 ) \]
\[o_{48} + 2o_{57} + 2o_{64} + 2o_{66} = \sum\limits_{x,t,u,v:P_{10} (x,t,u,v)} ( c( x, v ) - 1 ) \]
\[2o_{49} + 2o_{54} = \sum\limits_{x,t,u,v:P_{6} (x,t,u,v)} ( c( x, u, v ) - 1 ) \]
\[3o_{50} + 2o_{63} + o_{68} = \sum\limits_{x,t,u,v:P_{8} (x,t,u,v)} ( c( x, u ) - 2 ) \]
\[o_{51} + o_{59} + 4o_{62} + 4o_{65} = \sum\limits_{x,t,u,v:P_{9} (x,t,u,v)} ( c( x, u ) - 1 ) + ( c( x, v ) - 1 ) \]
\[2o_{52} + o_{59} = \sum\limits_{x,t,u,v:P_{4} (x,t,u,v)} c( x, t, v ) \]
\[o_{53} + 2o_{63} + 2o_{64} + 2o_{68} = \sum\limits_{x,t,u,v:P_{8} (x,t,u,v)} c( x, t ) + c( x, v ) \]
\[2o_{54} + 2o_{65} + o_{66} + 3o_{70} = \sum\limits_{x,t,u,v:P_{12} (x,t,u,v)} ( c( t, v ) - 2 ) \]
\[3o_{55} + 2o_{67} + 2o_{71} = \sum\limits_{x,t,u,v:P_{13} (x,t,u,v)} ( c( x, v ) - 2 ) \]
\[3o_{56} + 2o_{65} = \sum\limits_{x,t,u,v:P_{9} (x,t,u,v)} c( t, u, v ) \]
\[2o_{57} + 2o_{66} = \sum\limits_{x,t,u,v:P_{10} (x,t,u,v)} c( x, t, v ) \]
\[o_{58} + o_{67} + 2o_{71} + 4o_{72} = \sum\limits_{x,t,u,v:P_{14} (x,t,u,v)} ( c( x ) - 3 ) \]
\[o_{59} + 2o_{66} = \sum\limits_{x,t,u,v:P_{10} (x,t,u,v)} c( t, u, v ) \]
\[o_{60} + 2o_{66} = \sum\limits_{x,t,u,v:P_{10} (x,t,u,v)} c( x, t, u ) \]
\[2o_{61} + 2o_{67} = \sum\limits_{x,t,u,v:P_{11} (x,t,u,v)} c( x, t, u ) + c( x, u, v ) \]
\[2o_{62} + 2o_{65} = \sum\limits_{x,t,u,v:P_{9} (x,t,u,v)} ( c( x, u, v ) - 1 ) \]
\[o_{63} + o_{67} = \sum\limits_{x,t,u,v:P_{11} (x,t,u,v)} ( c( t, u, v ) - 1 ) \]
\[o_{64} + o_{68} = \sum\limits_{x,t,u,v:P_{8} (x,t,u,v)} c( x, t, v ) \]
\[2o_{65} + 3o_{70} = \sum\limits_{x,t,u,v:P_{12} (x,t,u,v)} c( t, u, v ) \]
\[o_{66} + 3o_{70} + 2o_{71} + 12o_{72} = \sum\limits_{x,t,u,v:P_{14} (x,t,u,v)} ( c( t, u ) - 2 ) + ( c( t, v ) - 2 ) + ( c( u, v ) - 2 ) \]
\[o_{67} + 4o_{71} + 12o_{72} = \sum\limits_{x,t,u,v:P_{14} (x,t,u,v)} ( c( x, t ) - 2 ) + ( c( x, u ) - 2 ) + ( c( x, v ) - 2 ) \]
\[o_{68} + 2o_{71} = \sum\limits_{x,t,u,v:P_{13} (x,t,u,v)} ( c( t, u, v ) - 1 ) \]
\[4o_{69} + 2o_{71} = \sum\limits_{x,t,u,v:P_{13} (x,t,u,v)} ( c( x, t, u ) - 1 ) \]
\[o_{70} + 4o_{72} = \sum\limits_{x,t,u,v:P_{14} (x,t,u,v)} ( c( t, u, v ) - 1 ) \]
\[2o_{71} + 12o_{72} = \sum\limits_{x,t,u,v:P_{14} (x,t,u,v)} ( c( x, t, u ) - 1 ) + ( c( x, t, v ) - 1 ) + ( c( x, u, v ) - 1 ) \]

